thx claude code

new/proof/github_com/sanjit_bhat/pav/ktcore_proof/serde.v
@@ -89,4 +89,84 @@ Proof. Admitted.
 End proof.
 End VrfSig.
 
+Module LinkSig.
+Record t :=
+  mk' {
+    SigTag: w8;
+    Epoch: w64;
+    Link: list w8;
+  }.
+
+Definition encodes (obj : t) (enc : list w8) : Prop :=
+  sint.Z (W64 (length obj.(Link))) = length obj.(Link) ∧
+
+  enc = [obj.(SigTag)] ++ u64_le obj.(Epoch) ++
+    u64_le (length obj.(Link)) ++ obj.(Link).
+
+Lemma inj {obj0 obj1 enc0 enc1 tail0 tail1} :
+  enc0 ++ tail0 = enc1 ++ tail1 →
+  encodes obj0 enc0 →
+  encodes obj1 enc1 →
+  obj0 = obj1 ∧ enc0 = enc1 ∧ tail0 = tail1.
+Proof. Admitted.
+
+Section proof.
+Context `{hG: heapGS Σ, !ffi_semantics _ _, !globalsGS Σ} {go_ctx : GoContext}.
+
+Definition own ptr obj d : iProp Σ :=
+  ∃ sl_Link,
+  "Hstruct" ∷ ptr ↦{d} (ktcore.LinkSig.mk obj.(SigTag) obj.(Epoch) sl_Link) ∗
+
+  "Hsl_Link" ∷ sl_Link ↦*{d} obj.(Link).
+
+Definition wish b obj tail : iProp Σ :=
+  ∃ enc,
+  "%Henc_obj" ∷ ⌜encodes obj enc⌝ ∗
+  "%Heq_tail" ∷ ⌜b = enc ++ tail⌝.
+
+Lemma wish_det b obj0 obj1 tail0 tail1 :
+  wish b obj0 tail0 -∗
+  wish b obj1 tail1 -∗
+  ⌜obj0 = obj1 ∧ tail0 = tail1⌝.
+Proof. Admitted.
+
+Lemma wp_enc sl_b b ptr_obj obj d :
+  {{{
+    is_pkg_init ktcore ∗
+    "Hsl_b" ∷ sl_b ↦* b ∗
+    "Hcap_b" ∷ own_slice_cap w8 sl_b 1 ∗
+    "Hown_obj" ∷ own ptr_obj obj d
+  }}}
+  @! ktcore.LinkSigEncode #sl_b #ptr_obj
+  {{{
+    sl_b' enc, RET #sl_b';
+    "Hsl_b" ∷ sl_b' ↦* (b ++ enc) ∗
+    "Hcap_b" ∷ own_slice_cap w8 sl_b' 1 ∗
+    "Hown_obj" ∷ own ptr_obj obj d ∗
+    "%Henc" ∷ ⌜encodes obj enc⌝
+  }}}.
+Proof. Admitted.
+
+Lemma wp_dec sl_b d b :
+  {{{
+    is_pkg_init ktcore ∗
+    "Hsl_b" ∷ sl_b ↦*{d} b
+  }}}
+  @! ktcore.LinkSigDecode #sl_b
+  {{{
+    ptr_obj sl_tail err, RET (#ptr_obj, #sl_tail, #err);
+    match err with
+    | true => ¬ ∃ obj tail, wish b obj tail
+    | false =>
+      ∃ obj tail,
+      "#Hwish" ∷ wish b obj tail ∗
+      "Hown_obj" ∷ own ptr_obj obj d ∗
+      "Hsl_tail" ∷ sl_tail ↦*{d} tail
+    end
+  }}}.
+Proof. Admitted.
+
+End proof.
+End LinkSig.
+
 End ktcore.
